src/3d/Options.fsti
@@ -24,3 +24,5 @@ val get_clang_format_executable : unit -> ML string
 val get_cleanup : unit -> ML bool
 
 val get_skip_makefiles : unit -> ML bool
+
+val get_no_everparse_h : unit -> ML bool
